Execution_resources/for_all_correctness.v
@@ -12,372 +12,6 @@ Fixpoint forall_no_error (e : execution_resource) (d : dimension) : Prop :=
   | _ => for_all e d <> Error
 end.
 
-Lemma forall_block_x :
-  forall x y z i n b, count i (thread_set_3xyz x y z (fun x : ThreadId_t => x :: []) b) n ->
-            count i (zip (buildList x (fun i0 : nat => thread_set_3xyz 1 y z (fun x0 : ThreadId_t => x0 :: [])
-                    (fun _ j k : nat => b i0 j k)))) n.
-Proof.
-  intros.
-  generalize dependent n. induction x; intros. destruct y; apply H.
-  simpl in *. destruct y,z.
-    simpl in *. rewrite blockempty. apply H. reflexivity.
-    simpl in *. rewrite blockempty. apply H. reflexivity.
-    simpl in *. rewrite blockempty. apply H. reflexivity.
-    simpl in *. apply cat_count_rev with (l1 := b x y z
-    :: (thread_set_1z (S x) (S y) z (fun x : ThreadId_t => x :: []) b) ++
-    thread_set_2yz (S x) y (S z) (fun x : ThreadId_t => x :: []) b) in H.
-    destruct H as [m1 [m2 [H [H' H2]]]]. subst.
-    apply cat_count with (l1 := b x y z
-        :: ((thread_set_1z 1 (S y) z (fun x0 : ThreadId_t => x0 :: []) (fun _ j k : nat => b x j k) ++
-        thread_set_2yz 1 y (S z) (fun x0 : ThreadId_t => x0 :: []) (fun _ j k : nat => b x j k)) ++ [])).
-    rewrite block_ok_yz.
-    rewrite block_ok_yz in H.
-    apply cat_count_rev with (l1 := b x y z
-    :: thread_set_1z (S x) (S y) z (fun x : ThreadId_t => x :: []) b) in H.
-    destruct H as [m1' [m2' [H [H1 H2]]]]. subst.
-    rewrite cat_empty.
-    apply cat_count with (l1 := b x y z
-    :: thread_set_1z 1 (S y) z (fun x0 : ThreadId_t => x0 :: []) (fun _ j k : nat => b x j k)).
-    rewrite block_ok_z. rewrite block_ok_z in H.
-    apply H.
-    simpl.
-    clear H. clear H'. clear IHx. generalize dependent m2'. induction y.
-        intros. apply H1. simpl. intros.
-        apply cat_count_rev with (l1 := b x y z
-        :: buildList z (fun k : nat => b x y k)) in H1.
-        destruct H1 as [m [m' [H1 [H2 H3]]]]. subst.
-        apply cat_count with (l1 := b x y z
-        :: buildList z (fun k : nat => b x y k)).
-        apply H1. apply IHy. apply H2.
-    apply IHx in H'.
-    apply H'.
-Qed.
-
-Lemma forall_block_y :
-  forall x y z i n b, count i (thread_set_3xyz x y z (fun x : ThreadId_t => x :: []) b) n ->
-            count i (zip (buildList y (fun i0 : nat => thread_set_3xyz x 1 z (fun x0 : ThreadId_t => x0 :: [])
-                    (fun i1 _ k : nat => b i1 i0 k)))) n.
-Proof.
-  intros. apply transpose_xy_block in H.
-  generalize dependent n. induction y; intros. destruct x; apply H.
-  simpl in *. destruct x,z.
-    simpl in *. rewrite blockempty. apply H. reflexivity.
-    simpl in *. rewrite blockempty. apply H. reflexivity.
-    simpl in *. rewrite blockempty. apply H. reflexivity.
-    simpl in *. apply cat_count_rev with (l1 := b x y z
-    :: (thread_set_1z (S x) (S y) z (fun x : ThreadId_t => x :: []) b) ++
-    thread_set_2xz x (S y) (S z) (fun x : ThreadId_t => x :: []) b) in H.
-    destruct H as [m1 [m2 [H [H' H2]]]]. subst.
-    apply cat_count with (l1 := b x y z
-    :: ((thread_set_1z (S x) 1 z (fun x0 : ThreadId_t => x0 :: []) (fun i1 _ k : nat => b i1 y k) ++ []) ++
-    thread_set_3xyz x 1 (S z) (fun x0 : ThreadId_t => x0 :: []) (fun i1 _ k : nat => b i1 y k))).
-    rewrite block_ok_xyz.
-    rewrite block_ok_xz in H.
-    apply cat_count_rev with (l1 := b x y z
-    :: thread_set_1z (S x) (S y) z (fun x : ThreadId_t => x :: []) b) in H.
-    destruct H as [m1' [m2' [H [H1 H2]]]]. subst.
-    rewrite cat_empty.
-    apply cat_count with (l1 := b x y z
-    :: thread_set_1z (S x) 1 z (fun x0 : ThreadId_t => x0 :: []) (fun i1 _ k : nat => b i1 y k)).
-    rewrite block_ok_z. rewrite block_ok_z in H.
-    apply H.
-    simpl.
-    assert (forall z, zip (buildList x (fun i0 : nat =>
-        zip (buildList 1 (fun _ : nat => buildList (S z) (fun k : nat => b i0 y k))))) =
-        zip (buildList x (fun j : nat => buildList (S z) (fun k : nat => b j y k)))).
-        clear. induction x.
-        reflexivity. simpl. intros.
-        simpl in IHx. rewrite IHx.
-        rewrite cat_empty. reflexivity.
-    simpl in H0.
-    rewrite H0. apply H1.
-    apply IHy in H'.
-    apply H'.
-Qed.
-
-Lemma forall_block_z :
-  forall x y z i n b, count i (thread_set_3xyz x y z (fun x : ThreadId_t => x :: []) b) n ->
-            count i (zip (buildList z
-           (fun i0 : nat => thread_set_3xyz x y 1 (fun x0 : ThreadId_t => x0 :: [])
-                    (fun i1 j k : nat => b i1 j i0)))) n.
-Proof.
-intros. apply transpose_xz_block in H.
-generalize dependent n. induction z; intros. destruct x,y; apply H.
-simpl in *. destruct x,y.
-  simpl in *. rewrite blockempty. apply H. reflexivity.
-  simpl in *. rewrite blockempty. apply H. reflexivity.
-  simpl in *. rewrite blockempty. apply H. reflexivity.
-  simpl in *. apply cat_count_rev with (l1 := b x y z
-  :: (thread_set_1y (S x) y (S z) (fun x : ThreadId_t => x :: []) b) ++
-  thread_set_2xy x (S y) (S z) (fun x : ThreadId_t => x :: []) b) in H.
-  destruct H as [m1 [m2 [H [H' H2]]]]. subst.
-  apply cat_count with (l1 := b x y z
-  :: (thread_set_2yz (S x) y 1 (fun x0 : ThreadId_t => x0 :: []) (fun i1 j _ : nat => b i1 j z) ++
-  thread_set_3xyz x (S y) 1 (fun x0 : ThreadId_t => x0 :: []) (fun i1 j _ : nat => b i1 j z))).
-  rewrite block_ok_xyz.
-  rewrite block_ok_xy in H.
-  apply cat_count_rev with (l1 := b x y z
-  :: thread_set_1y (S x) y (S z) (fun x : ThreadId_t => x :: []) b) in H.
-  destruct H as [m1' [m2' [H [H1 H2]]]]. subst.
-  apply cat_count with (l1 := b x y z
-  :: thread_set_2yz (S x) y 1 (fun x0 : ThreadId_t => x0 :: []) (fun i1 j k : nat => b i1 j z)).
-  rewrite block_ok_yz. rewrite block_ok_y in H.
-  simpl.
-  assert (forall n, count i (b x y z :: buildList y (fun k : nat => b x k z)) n ->
-  count i (b x y z :: zip (buildList y (fun j : nat => b x j z :: []))) n).
-    clear. induction y. intros. apply H. intros. simpl in *. inversion H; clear H; subst.
-    apply cons_eq; apply IHy; apply H4.
-    apply cons_neq. apply IHy; apply H4. apply Hneq.
-  apply H0 in H.
-  apply H.
-  simpl.
-  assert (forall n, count i (zip (buildList x (fun j : nat => buildList (S y) (fun k : nat => b j k z)))) n ->
-  count i (zip (buildList x (fun i0 : nat => zip (buildList (S y) (fun j : nat => b i0 j z :: []))))) n).
-    clear. induction x. intros. apply H. intros. simpl in *. inversion H; clear H; subst.
-    apply cons_eq. rewrite zip_ok. apply cat_count_rev in H4.
-    destruct H4 as [m [m' [H1 [H2 H3]]]]. subst.
-    apply cat_count.
-    apply H1. apply IHx; apply H2.
-    apply cons_neq.
-    rewrite zip_ok. apply cat_count_rev in H4.
-    destruct H4 as [m [m' [H1 [H2 H3]]]]. subst.
-    apply cat_count.
-    apply H1. apply IHx; apply H2. apply Hneq.
-  apply H0 in H1.
-  apply H1.
-  apply IHz in H'.
-  apply H'.
-Qed.
-
-Lemma forall_grid_x :
-  forall x y z x' y' z' i n g, count i (thread_set_3xyz x y z (fun b => thread_set_3xyz x' y' z' (fun x : ThreadId_t => x :: []) b) g) n ->
-            count i (zip (buildList x (fun i0 : nat => thread_set_3xyz 1 y z (fun b => thread_set_3xyz x' y' z' (fun x : ThreadId_t => x :: []) b)
-                    (fun _ j k : nat => g i0 j k)))) n.
-Proof.
-  intros.
-  generalize dependent n. induction x; intros. destruct y; apply H.
-  simpl in *. destruct y,z.
-    simpl in *. rewrite blockempty. apply H. reflexivity.
-    simpl in *. rewrite blockempty. apply H. reflexivity.
-    simpl in *. rewrite blockempty. apply H. reflexivity.
-    simpl in *.
-    apply cat_count_rev in H.
-    destruct H as [m01 [m02 [H [H01 H02]]]]. subst.
-    apply cat_count_rev in H.
-    destruct H as [m11 [m12 [H [H11 H12]]]]. subst.
-    apply cat_count_rev in H.
-    destruct H as [m21 [m22 [H [H21 H2]]]]. subst.
-    repeat (rewrite cat_empty).
-    apply cat_count.
-    apply cat_count.
-    apply cat_count.
-    apply H.
-    rewrite grid_ok_z.
-    rewrite grid_ok_z in H21.
-    apply H21.
-    rewrite grid_ok_yz.
-    rewrite grid_ok_yz in H11.
-    apply H11.
-    clear H. clear H11. clear H21. clear IHx. generalize dependent m02. induction x.
-        intros. apply H01. simpl. intros.
-        apply cat_count_rev in H01.
-        destruct H01 as [m [m' [H1 [H2 H3]]]]. subst.
-        repeat (rewrite cat_empty).
-        apply cat_count.
-        rewrite grid_ok_z in H1.
-        rewrite grid_ok_yz in H1.
-        rewrite grid_ok_z.
-        rewrite grid_ok_yz.
-        apply H1. apply IHx.
-    apply H2.
-Qed.
-
-Lemma forall_grid_y :
-  forall x y z x' y' z' i n g, count i (thread_set_3xyz x y z (fun b => thread_set_3xyz x' y' z' (fun x : ThreadId_t => x :: []) b) g) n ->
-            count i (zip (buildList y (fun i0 : nat => thread_set_3xyz x 1 z (fun b => thread_set_3xyz x' y' z' (fun x : ThreadId_t => x :: []) b)
-                    (fun i1 _ k : nat => g i1 i0 k)))) n.
-Proof.
-  intros. apply transpose_xy_grid in H.
-  generalize dependent n. induction y; intros. destruct x; apply H.
-  simpl in *. destruct x,z.
-    simpl in *. rewrite blockempty. apply H. reflexivity.
-    simpl in *. rewrite blockempty. apply H. reflexivity.
-    simpl in *. rewrite blockempty. apply H. reflexivity.
-    simpl in *.
-    apply cat_count_rev in H.
-    destruct H as [m01 [m02 [H [H01 H02]]]]. subst.
-    apply cat_count_rev in H.
-    destruct H as [m11 [m12 [H [H11 H12]]]]. subst.
-    apply cat_count_rev in H.
-    destruct H as [m21 [m22 [H [H21 H2]]]]. subst.
-    repeat (rewrite cat_empty).
-    apply cat_count.
-    apply cat_count.
-    apply cat_count.
-    apply H.
-    rewrite grid_ok_z.
-    rewrite grid_ok_z in H21.
-    apply H21.
-    rewrite grid_ok_xyz.
-    rewrite grid_ok_xz in H11.
-    clear H. clear H01. clear H21. clear IHy. generalize dependent m12. induction x.
-        intros. apply H11. simpl. intros.
-        apply cat_count_rev in H11.
-        destruct H11 as [m [m' [H1 [H2 H3]]]]. subst.
-        repeat (rewrite cat_empty).
-        apply cat_count. apply H1.
-        apply IHx. apply H2.
-    clear H. clear H11. clear H21. clear IHy. generalize dependent m02. induction y.
-        intros. apply H01. simpl. intros.
-        apply cat_count_rev in H01.
-        destruct H01 as [m [m' [H1 [H2 H3]]]]. subst.
-        repeat (rewrite cat_empty).
-        apply cat_count.
-        rewrite grid_ok_z in H1.
-        rewrite grid_ok_xz in H1.
-        rewrite grid_ok_z.
-        rewrite grid_ok_xyz.
-        apply cat_count_rev in H1.
-        destruct H1 as [m1 [m2 [H1 [H2' H3]]]]. subst.
-        repeat (rewrite cat_empty).
-        apply cat_count.
-        apply H1.
-        apply cat_count_rev in H1.
-        destruct H1 as [m1' [m2' [H1 [H2'' H3]]]]. subst.
-        repeat (rewrite cat_empty).
-        clear H2. clear H2''. clear H1. clear IHy.
-        clear m12. clear m21. clear m'. clear m1'. clear m2'.
-        generalize dependent m2. induction x.
-          intros. apply H2'.
-          intros. simpl in *.
-          apply cat_count_rev in H2'.
-          destruct H2' as [m01 [m02 [H [H01 H02]]]]. subst.
-          apply cat_count_rev in H.
-          destruct H as [m11 [m12 [H [H11 H12]]]]. subst.
-          repeat (rewrite cat_empty).
-          apply cat_count. apply cat_count.
-          apply H.
-          apply H11.
-          apply IHx. apply H01.
-    apply IHy.
-    apply H2.
-Qed.
-
-Lemma forall_grid_z :
-  forall x y z x' y' z' i n g, count i (thread_set_3xyz x y z (fun b => thread_set_3xyz x' y' z' (fun x : ThreadId_t => x :: []) b) g) n ->
-            count i (zip (buildList z (fun i0 : nat => thread_set_3xyz x y 1 (fun b => thread_set_3xyz x' y' z' (fun x : ThreadId_t => x :: []) b)
-                    (fun i j k : nat => g i j i0)))) n.
-Proof.
-  intros. apply transpose_xz_grid in H.
-  generalize dependent n. induction z; intros. destruct x,y; apply H.
-  simpl in *. destruct x,y.
-    simpl in *. rewrite blockempty. apply H. reflexivity.
-    simpl in *. rewrite blockempty. apply H. reflexivity.
-    simpl in *. rewrite blockempty. apply H. reflexivity.
-    simpl in *.
-    apply cat_count_rev in H.
-    destruct H as [m01 [m02 [H [H01 H02]]]]. subst.
-    apply cat_count_rev in H.
-    destruct H as [m11 [m12 [H [H11 H12]]]]. subst.
-    apply cat_count_rev in H.
-    destruct H as [m21 [m22 [H [H21 H2]]]]. subst.
-    repeat (rewrite cat_empty).
-    apply cat_count.
-    apply cat_count.
-    apply cat_count.
-    apply H.
-    rewrite grid_ok_yz.
-    rewrite grid_ok_y in H21.
-    clear H. clear H11. clear H01. clear IHz. generalize dependent m22.
-    clear m02. clear m12. induction y.
-      intros. apply H21.
-      intros. simpl in *.
-      apply cat_count_rev in H21.
-      destruct H21 as [m01 [m02 [H [H01 H02]]]]. subst.
-      repeat (rewrite cat_empty).
-      apply cat_count.
-      apply H.
-      apply IHy. apply H01.
-    rewrite grid_ok_xyz.
-    rewrite grid_ok_xy in H11.
-    clear H. clear H21. clear H01. clear IHz. generalize dependent m12.
-    clear m02. clear m22. induction x.
-      intros. apply H11.
-      intros. simpl in *.
-      apply cat_count_rev in H11.
-      destruct H11 as [m01 [m02 [H [H01 H02]]]]. subst.
-      apply cat_count_rev in H.
-      destruct H as [m11 [m12 [H [H11 H12]]]]. subst.
-      repeat (rewrite cat_empty).
-      apply cat_count.
-      apply cat_count.
-      apply H.
-      clear H01. clear H. clear IHx.
-      clear m21. clear m02. clear m11. generalize dependent m12.
-      induction y.
-        intros. apply H11.
-        intros. simpl in *.
-        apply cat_count_rev in H11.
-        destruct H11 as [m01 [m02 [H [H01 H02]]]]. subst.
-        repeat (rewrite cat_empty).
-        apply cat_count.
-        apply H.
-        apply IHy. apply H01.
-      apply IHx. apply H01.
-    clear H. clear H11. clear H21. clear IHz. generalize dependent m02.
-    clear m12. clear m21. clear m22. induction z.
-        intros. apply H01.
-        simpl. intros.
-        apply cat_count_rev in H01.
-        destruct H01 as [m01 [m02' [H [H01 H02]]]]. subst.
-        apply cat_count_rev in H.
-        destruct H as [m11 [m12 [H [H11 H12]]]]. subst.
-        apply cat_count_rev in H.
-        destruct H as [m21 [m22 [H [H21 H22]]]]. subst.
-        repeat (rewrite cat_empty).
-        apply cat_count.
-        apply cat_count.
-        apply cat_count.
-        apply H.
-        rewrite grid_ok_y in H21.
-        rewrite grid_ok_yz.
-        clear H. clear H11. clear H01. clear m02'. clear m12. clear m21.
-        generalize dependent m22. clear IHz. induction y.
-          intros. apply H21.
-          intros. simpl in *.
-          apply cat_count_rev in H21.
-          destruct H21 as [m01 [m02 [H [H01 H02]]]]. subst.
-          repeat (rewrite cat_empty).
-          apply cat_count.
-          apply H.
-          apply IHy. apply H01.
-        rewrite grid_ok_xyz.
-        rewrite grid_ok_xy in H11.
-        clear H. clear H21. clear H01. clear m02'. clear m22. clear m21.
-        generalize dependent m12. clear IHz. induction x.
-          intros. apply H11.
-          intros. simpl in *.
-          apply cat_count_rev in H11.
-          destruct H11 as [m01 [m02 [H [H01 H02]]]]. subst.
-          apply cat_count_rev in H.
-          destruct H as [m11 [m12' [H [H11 H12]]]]. subst.
-          repeat (rewrite cat_empty).
-          apply cat_count. apply cat_count.
-          apply H.
-          clear H. clear H01. clear m02. clear m11.
-          generalize dependent m12'. clear IHx. induction y.
-            intros. apply H11.
-          intros. simpl in *.
-          apply cat_count_rev in H11.
-          destruct H11 as [m01 [m02 [H [H01 H02]]]]. subst.
-          repeat (rewrite cat_empty).
-          apply cat_count.
-          apply H.
-          apply IHy. apply H01.
-        apply IHx. apply H01.
-    apply IHz. apply H01.
-Qed.
-
 Proposition induction_step_collection_forall :
   forall i n v n0 d,
 (forall n' n0, n' < n -> count i (thread_set' (v n')) n0 ->
@@ -423,353 +57,68 @@ Proposition for_all_correct :
 Proof.
   induction e; intros; try (exfalso; apply H; reflexivity).
   - simpl in *.
-    destruct d; try (exfalso; apply H; reflexivity).
-    simpl. clear H. induction Warp_size. apply H0. apply IHn.
-  - destruct d.
-    + destruct shp as [p z]. destruct p as [x y].
-    destruct id as [p iz]. destruct p as [ix iy].
-    destruct x,y,z.
-      * apply H0.
-      * destruct z; apply H0.
-      * destruct y; apply H0.
-      * destruct y; destruct z; apply H0.
-      * inversion H0. subst.
-        destruct x. apply H0.
-        simpl. clear. induction x.
-        ** apply empty.
-        ** simpl. apply IHx.
-      * inversion H0. subst.
-        destruct x. destruct z; apply H0.
-        simpl. clear. induction x.
-        ** destruct z; apply empty.
-        ** simpl. destruct z; apply IHx.
-      * inversion H0. subst.
-        destruct x. destruct y; apply H0.
-        simpl. clear. induction x.
-        ** destruct y; apply empty.
-        ** simpl. destruct y; apply IHx.
-      * destruct x.
-        ** exfalso; apply H. simpl. destruct y,z;try reflexivity.
-        ** destruct y,z.
-          -- simpl in *. rewrite block_ok_xyz in H0. apply H0.
-        -- simpl in *.
-              assert (count i (thread_set_3xyz (S (S x)) 1 (S (S z)) (fun x0 : ThreadId_t => x0 :: []) b) m).
-              simpl. apply H0. apply forall_block_x in H1. apply H1.
-        -- simpl in *.
-              assert (count i (thread_set_3xyz (S (S x)) (S (S y)) 1 (fun x0 : ThreadId_t => x0 :: []) b) m).
-              simpl. apply H0. apply forall_block_x in H1. apply H1.
-        -- simpl in *.
-              assert (count i (thread_set_3xyz (S (S x)) (S (S y)) (S (S z)) (fun x0 : ThreadId_t => x0 :: []) b) m).
-              simpl. apply H0. apply forall_block_x in H1. apply H1.
-    + destruct shp as [p z]. destruct p as [x y].
-    destruct id as [p iz]. destruct p as [ix iy].
-    destruct y,x,z.
-      * apply H0.
-      * destruct z; apply H0.
-      * destruct x; apply H0.
-      * destruct x; destruct z; apply H0.
-      * inversion H0. subst.
-        destruct y. apply H0.
-        simpl. clear. induction y.
-        ** apply empty.
-        ** simpl. apply IHy.
-      * inversion H0. subst.
-        destruct y. destruct z; apply H0.
-        simpl. clear. induction y.
-        ** destruct z; apply empty.
-        ** simpl. destruct z; apply IHy.
-      * inversion H0. subst.
-        destruct y. destruct x; apply H0.
-        simpl. clear. induction y.
-        ** destruct x; apply empty.
-        ** simpl. destruct x; apply IHy.
-      * destruct y.
-        ** exfalso; apply H. simpl. destruct x,z;try reflexivity.
-        ** destruct x,z.
-          -- simpl in *. rewrite block_ok_yz in H0. rewrite cat_empty in H0. apply H0.
-          -- simpl in *.
-                assert (count i (thread_set_3xyz 1 (S (S y)) (S (S z)) (fun x0 : ThreadId_t => x0 :: []) b) m).
-                simpl. apply H0. apply forall_block_y in H1. apply H1.
-          -- simpl in *.
-                assert (count i (thread_set_3xyz (S (S x)) (S (S y)) 1 (fun x0 : ThreadId_t => x0 :: []) b) m).
-                simpl. apply H0. apply forall_block_y in H1. apply H1.
-          -- simpl in *.
-                assert (count i (thread_set_3xyz (S (S x)) (S (S y)) (S (S z)) (fun x0 : ThreadId_t => x0 :: []) b) m).
-                simpl. apply H0. apply forall_block_y in H1. apply H1.
-    + destruct shp as [p z]. destruct p as [x y].
-    destruct id as [p iz]. destruct p as [ix iy].
-    destruct z,x,y.
-      * apply H0.
-      * destruct y; apply H0.
-      * destruct x; apply H0.
-      * destruct x; destruct y; apply H0.
-      * inversion H0. subst.
-        destruct z. apply H0.
-        simpl. clear. induction z.
-        ** apply empty.
-        ** simpl. apply IHz.
-      * inversion H0. subst.
-        destruct z. destruct y; apply H0.
-        simpl. clear. induction z.
-        ** destruct y; apply empty.
-        ** simpl. destruct y; apply IHz.
-      * inversion H0. subst.
-        destruct z. destruct x; apply H0.
-        simpl. clear. induction z.
-        ** destruct x; apply empty.
-        ** simpl. destruct x; apply IHz.
-      * destruct z.
-        ** exfalso; apply H. simpl. destruct x,y;try reflexivity.
-        ** destruct x,y.
-          -- simpl in *. rewrite block_ok_z in H0. rewrite cat_empty in H0. rewrite cat_empty in H0.
-          assert (forall i m, count i (buildList z (fun k : nat => b 0 0 k)) m -> count i (zip (buildList z (fun i0 : nat => b 0 0 i0 :: []))) m).
-            clear. induction z. intros. apply H. simpl. intros. inversion H; clear H; subst; try (apply cons_eq); try (apply cons_neq); try (apply IHz; apply H4). apply Hneq.
-          inversion H0; inversion H6; subst; clear H0; clear H6;
-          repeat (repeat (apply cons_eq); try (apply cons_neq)); try (apply H1; apply H11).
-          apply Hneq. apply Hneq. apply Hneq0. apply Hneq.
-        -- simpl in *.
-              assert (count i (thread_set_3xyz 1 (S (S y)) (S (S z)) (fun x0 : ThreadId_t => x0 :: []) b) m).
-              simpl. apply H0. apply forall_block_z in H1. apply H1.
-        -- simpl in *.
-              assert (count i (thread_set_3xyz (S (S x)) 1 (S (S z)) (fun x0 : ThreadId_t => x0 :: []) b) m).
-              simpl. apply H0. apply forall_block_z in H1. apply H1.
-        -- simpl in *.
-              assert (count i (thread_set_3xyz (S (S x)) (S (S y)) (S (S z)) (fun x0 : ThreadId_t => x0 :: []) b) m).
-              simpl. apply H0. apply forall_block_z in H1. apply H1.
-  - destruct d.
-    + destruct shp as [p z]. destruct p as [x y].
-    destruct shp' as [p z']. destruct p as [x' y'].
-    destruct x,y,z.
-      * apply H0.
-      * destruct z; apply H0.
-      * destruct y; apply H0.
-      * destruct y; destruct z; apply H0.
-      * inversion H0. subst.
-        destruct x. apply H0.
-        simpl. clear. induction x.
-        ** apply empty.
-        ** simpl. apply IHx.
-      * inversion H0. subst.
-        destruct x. destruct z; apply H0.
-        simpl. clear. induction x.
-        ** destruct z; apply empty.
-        ** simpl. destruct z; apply IHx.
-      * inversion H0. subst.
-        destruct x. destruct y; apply H0.
-        simpl. clear. induction x.
-        ** destruct y; apply empty.
-        ** simpl. destruct y; apply IHx.
-      * destruct x.
-        ** exfalso; apply H. simpl. destruct y,z;try reflexivity.
-        ** destruct y,z.
-          -- simpl in *. rewrite grid_ok_xyz in H0. repeat (rewrite block_ok_xyz in H0). repeat (rewrite block_ok_xyz).
-             simpl in H0. repeat (rewrite cat_empty in H0).
-             apply cat_count_rev in H0; destruct H0 as [m1 [m2 [H0 [H1 H2]]]]; subst.
-             apply cat_count_rev in H1; destruct H1 as [m3 [m4 [H1 [H2 H3]]]]; subst.
-             apply cat_count. apply H0.
-             apply cat_count. apply H1.
-             clear H0. clear H1. clear H.
-             generalize dependent m4. induction x.
-                ++ intros. apply H2.
-                ++ simpl in *. intros. repeat (rewrite cat_empty in H2).
-                apply cat_count_rev in H2; destruct H2 as [m [m' [H0 [H1 H2]]]]; subst.
-                apply cat_count. apply H0.
-                apply IHx in H1. apply H1.
-        -- simpl in *.
-              assert (count i (thread_set_3xyz (S (S x)) 1 (S (S z)) (fun b => thread_set_3xyz x' y' z' (fun x : ThreadId_t => x :: []) b) g) m).
-              simpl. apply H0. apply forall_grid_x in H1. apply H1.
-        -- simpl in *.
-              assert (count i (thread_set_3xyz (S (S x)) (S (S y)) 1 (fun b => thread_set_3xyz x' y' z' (fun x : ThreadId_t => x :: []) b) g) m).
-              simpl. apply H0. apply forall_grid_x in H1. apply H1.
-        -- simpl in *.
-              assert (count i (thread_set_3xyz (S (S x)) (S (S y)) (S (S z)) (fun b => thread_set_3xyz x' y' z' (fun x : ThreadId_t => x :: []) b) g) m).
-              simpl. apply H0. apply forall_grid_x in H1. apply H1.
-    + destruct shp as [p z]. destruct p as [x y].
-    destruct shp' as [p z']. destruct p as [x' y'].
-    destruct y,x,z.
-      * apply H0.
-      * destruct z; apply H0.
-      * destruct x; apply H0.
-      * destruct x; destruct z; apply H0.
-      * inversion H0. subst.
-        destruct y. apply H0.
-        simpl. clear. induction y.
-        ** apply empty.
-        ** simpl. apply IHy.
-      * inversion H0. subst.
-        destruct y. destruct z; apply H0.
-        simpl. clear. induction y.
-        ** destruct z; apply empty.
-        ** simpl. destruct z; apply IHy.
-      * inversion H0. subst.
-        destruct y. destruct x; apply H0.
-        simpl. clear. induction y.
-        ** destruct x; apply empty.
-        ** simpl. destruct x; apply IHy.
-      * destruct y.
-        ** exfalso; apply H. simpl. destruct x,z;try reflexivity.
-        ** destruct x,z.
-          -- simpl in *. rewrite grid_ok_yz in H0. repeat (rewrite block_ok_xyz in H0). repeat (rewrite block_ok_xyz).
-             simpl in H0. repeat (rewrite cat_empty in H0).
-             apply cat_count_rev in H0; destruct H0 as [m1 [m2 [H0 [H1 H2]]]]; subst.
-             apply cat_count_rev in H1; destruct H1 as [m3 [m4 [H1 [H2 H3]]]]; subst.
-             apply cat_count. apply H0.
-             apply cat_count. apply H1.
-             clear H0. clear H1. clear H.
-             generalize dependent m4. induction y.
-                ++ intros. apply H2.
-                ++ simpl in *. intros. repeat (rewrite cat_empty in H2).
-                apply cat_count_rev in H2; destruct H2 as [m [m' [H0 [H1 H2]]]]; subst.
-                apply cat_count. apply H0.
-                apply IHy in H1. apply H1.
-        -- simpl in *.
-              assert (count i (thread_set_3xyz 1 (S (S y)) (S (S z)) (fun b => thread_set_3xyz x' y' z' (fun x : ThreadId_t => x :: []) b) g) m).
-              simpl. apply H0. apply forall_grid_y in H1. apply H1.
-        -- simpl in *.
-              assert (count i (thread_set_3xyz (S (S x)) (S (S y)) 1 (fun b => thread_set_3xyz x' y' z' (fun x : ThreadId_t => x :: []) b) g) m).
-              simpl. apply H0. apply forall_grid_y in H1. apply H1.
-        -- simpl in *.
-              assert (count i (thread_set_3xyz (S (S x)) (S (S y)) (S (S z)) (fun b => thread_set_3xyz x' y' z' (fun x : ThreadId_t => x :: []) b) g) m).
-              simpl. apply H0. apply forall_grid_y in H1. apply H1.
-    + destruct shp as [p z]. destruct p as [x y].
-    destruct shp' as [p z']. destruct p as [x' y'].
-    destruct z,x,y.
-      * apply H0.
-      * destruct y; apply H0.
-      * destruct x; apply H0.
-      * destruct x; destruct y; apply H0.
-      * inversion H0. subst.
-        destruct z. apply H0.
-        simpl. clear. induction z.
-        ** apply empty.
-        ** simpl. apply IHz.
-      * inversion H0. subst.
-        destruct z. destruct y; apply H0.
-        simpl. clear. induction z.
-        ** destruct y; apply empty.
-        ** simpl. destruct y; apply IHz.
-      * inversion H0. subst.
-        destruct z. destruct x; apply H0.
-        simpl. clear. induction z.
-        ** destruct x; apply empty.
-        ** simpl. destruct x; apply IHz.
-      * destruct z.
-        ** exfalso; apply H. simpl. destruct x,y;try reflexivity.
-        ** destruct x,y.
-          -- simpl in *. rewrite grid_ok_z in H0. repeat (rewrite block_ok_xyz in H0). repeat (rewrite block_ok_xyz).
-             simpl in H0. repeat (rewrite cat_empty in H0).
-             apply cat_count_rev in H0; destruct H0 as [m1 [m2 [H0 [H1 H2]]]]; subst.
-             apply cat_count_rev in H1; destruct H1 as [m3 [m4 [H1 [H2 H3]]]]; subst.
-             apply cat_count. apply H0.
-             apply cat_count. apply H1.
-             clear H0. clear H1. clear H.
-             generalize dependent m4. induction z.
-                ++ intros. apply H2.
-                ++ simpl in *. intros. repeat (rewrite cat_empty in H2).
-                apply cat_count_rev in H2; destruct H2 as [m [m' [H0 [H1 H2]]]]; subst.
-                apply cat_count. apply H0.
-                apply IHz in H1. apply H1.
-        -- simpl in *.
-              assert (count i (thread_set_3xyz 1 (S (S y)) (S (S z)) (fun b => thread_set_3xyz x' y' z' (fun x : ThreadId_t => x :: []) b) g) m).
-              simpl. apply H0. apply forall_grid_z in H1. apply H1.
-        -- simpl in *.
-              assert (count i (thread_set_3xyz (S (S x)) 1 (S (S z)) (fun b => thread_set_3xyz x' y' z' (fun x : ThreadId_t => x :: []) b) g) m).
-              simpl. apply H0. apply forall_grid_z in H1. apply H1.
-        -- simpl in *.
-              assert (count i (thread_set_3xyz (S (S x)) (S (S y)) (S (S z)) (fun b => thread_set_3xyz x' y' z' (fun x : ThreadId_t => x :: []) b) g) m).
-              simpl. apply H0. apply forall_grid_z in H1. apply H1.
-  - simpl in *.
     apply induction_step_collection_forall.
     intros.
     apply H with (m := n0).
     apply H0. apply H2. apply H3. apply H1.
+  - destruct d.
+    + simpl in *. clear H. clear H0.
+      generalize dependent m. induction x.
+      * intros. apply H1.
+      * intros. simpl in *. rewrite cat_empty. apply cat_count_rev in H1.
+      destruct H1 as [m1 [m2 [H1 [H2 H3]]]]; subst.
+      apply cat_count. apply H1. apply IHx. apply H2.
+    + simpl in *. apply transpose_lemma. clear H. clear H0.
+      generalize dependent m. induction x.
+      * intros. apply H1.
+      * intros. simpl in *. apply cat_count_rev in H1.
+      destruct H1 as [m1 [m2 [H1 [H2 H3]]]]; subst.
+      apply cat_count. clear H2. clear IHx.
+        generalize dependent m1. induction y. intros.
+            apply H1. intros. apply cat_count_rev in H1.
+        destruct H1 as [m1' [m2' [H1 [H2 H3]]]]; subst.
+        apply cat_count. rewrite cat_empty. apply H1. apply IHy.
+        apply H2.
+      apply IHx. apply H2.
+    + simpl in *. apply transpose_lemma. apply transpose_lemma'. clear H. clear H0.
+      generalize dependent m. induction x.
+      * intros. apply H1.
+      * intros. simpl in *. apply cat_count_rev in H1.
+      destruct H1 as [m1 [m2 [H1 [H2 H3]]]]; subst.
+      apply cat_count. clear H2. clear IHx.
+        generalize dependent m1. induction y. intros.
+          apply H1. intros. apply cat_count_rev in H1.
+          destruct H1 as [m1' [m2' [H1 [H2 H3]]]]; subst.
+          apply cat_count. clear H2. clear IHy.
+          generalize dependent m1'. induction z. intros.
+            apply H1. intros. apply cat_count_rev in H1.
+            destruct H1 as [m1'' [m2'' [H1 [H2 H3]]]]; subst.
+            apply cat_count. rewrite cat_empty. apply H1. apply IHz.
+            apply H2.
+        apply IHy. apply H2.
+      apply IHx. apply H2.
 Qed.
 
 Proposition for_all_error :
   forall e d,
   for_all e d = Error -> (
-  (d = _x /\ exists y z i b, e = block (1,y,z) i b) \/
-  (d = _x /\ exists y z i g, e = grid (1,y,z) i g) \/
-  (d = _y /\ exists x z i b, e = block (x,1,z) i b) \/
-  (d = _y /\ exists x z i g, e = grid (x,1,z) i g) \/
-  (d = _z /\ exists x y i b, e = block (x,y,1) i b) \/
-  (d = _z /\ exists x y i g, e = grid (x,y,1) i g) \/
-  (d <> _x /\ exists w, e = warp w) \/
+  (exists s i b, e = block s i b) \/
+  (exists s s' g, e = grid s s' g) \/
+  (exists w, e = warp w) \/
   (exists i, e = thread i) \/
   (exists i, e = lthread i) \/
   e = Error
 ).
 Proof.
-  destruct e,d; intros; simpl in *.
-  - right. right. right. right. right. right. right. left. exists t. reflexivity.
-  - right. right. right. right. right. right. right. left. exists t. reflexivity.
-  - right. right. right. right. right. right. right. left. exists t. reflexivity.
-  - right. right. right. right. right. right. right. right. left. exists t. reflexivity.
-  - right. right. right. right. right. right. right. right. left. exists t. reflexivity.
-  - right. right. right. right. right. right. right. right. left. exists t. reflexivity.
+  destruct e; intros; simpl in *.
+  - right. right. right. left. exists t. reflexivity.
+  - right. right. right. right. left. exists t. reflexivity.
+  - right. right. left. exists w. reflexivity.
+  - left. exists shp,id,b. reflexivity.
+  - right. left. exists shp,shp',g. reflexivity.
   - inversion H.
-  - right. right. right. right. right. right. left. split. intro. inversion H0. exists w. reflexivity.
-  - right. right. right. right. right. right. left. split. intro. inversion H0. exists w. reflexivity.
-  - destruct shp as [p z]. destruct p as [x y].
-    destruct id as [p idz]. destruct p as [idx idy]. destruct x.
-      * destruct y,z; try (destruct y); try (destruct z); inversion H.
-      * destruct x. destruct y,z; left; split; try (reflexivity).
-        + exists 0,0, (idx,idy,idz), b;reflexivity.
-        + exists 0,(S z), (idx,idy,idz), b;reflexivity.
-        + exists (S y),0, (idx,idy,idz), b;reflexivity.
-        + exists (S y),(S z), (idx,idy,idz), b;reflexivity.
-        + destruct y,z; try (destruct y); try (destruct z); inversion H.
-  - destruct shp as [p z]. destruct p as [x y].
-    destruct id as [p idz]. destruct p as [idx idy]. destruct y.
-      * destruct x,z; try (destruct x); try (destruct z); inversion H.
-      * destruct y. destruct x,z; right; right; left; split; try (reflexivity).
-        + exists 0,0, (idx,idy,idz), b;reflexivity.
-        + exists 0,(S z), (idx,idy,idz), b;reflexivity.
-        + exists (S x),0, (idx,idy,idz), b;reflexivity.
-        + exists (S x),(S z), (idx,idy,idz), b;reflexivity.
-        + destruct x,z; try (destruct x); try (destruct z); inversion H.
-  - destruct shp as [p z]. destruct p as [x y].
-    destruct id as [p idz]. destruct p as [idx idy]. destruct z.
-      * destruct x,y; try (destruct x); try (destruct y); inversion H.
-      * destruct z. destruct x,y; right; right; right; right; left; split; try (reflexivity).
-        + exists 0,0, (idx,idy,idz), b;reflexivity.
-        + exists 0,(S y), (idx,idy,idz), b;reflexivity.
-        + exists (S x),0, (idx,idy,idz), b;reflexivity.
-        + exists (S x),(S y), (idx,idy,idz), b;reflexivity.
-        + destruct x,y; try (destruct x); try (destruct y); inversion H.
-  - destruct shp as [p z]. destruct p as [x y].
-    destruct shp' as [p z']. destruct p as [x' y']. destruct x.
-      * destruct y,z; try (destruct y); try (destruct z); inversion H.
-      * destruct x. destruct y,z; right; left; split; try (reflexivity).
-        + exists 0,0, (x',y',z'), g;reflexivity.
-        + exists 0,(S z), (x',y',z'), g;reflexivity.
-        + exists (S y),0, (x',y',z'), g;reflexivity.
-        + exists (S y),(S z), (x',y',z'), g;reflexivity.
-        + destruct y,z; try (destruct y); try (destruct z); inversion H.
-  - destruct shp as [p z]. destruct p as [x y].
-    destruct shp' as [p z']. destruct p as [x' y']. destruct y.
-      * destruct x,z; try (destruct x); try (destruct z); inversion H.
-      * destruct y. destruct x,z; right; right; right; left; split; try (reflexivity).
-        + exists 0,0, (x',y',z'), g;reflexivity.
-        + exists 0,(S z), (x',y',z'), g;reflexivity.
-        + exists (S x),0, (x',y',z'), g;reflexivity.
-        + exists (S x),(S z), (x',y',z'), g;reflexivity.
-        + destruct x,z; try (destruct x); try (destruct z); inversion H.
-  - destruct shp as [p z]. destruct p as [x y].
-    destruct shp' as [p z']. destruct p as [x' y']. destruct z.
-      * destruct x,y; try (destruct x); try (destruct y); inversion H.
-      * destruct z. destruct x,y; right; right; right; right; right; left; split; try (reflexivity).
-        + exists 0,0, (x',y',z'), g;reflexivity.
-        + exists 0,(S y), (x',y',z'), g;reflexivity.
-        + exists (S x),0, (x',y',z'), g;reflexivity.
-        + exists (S x),(S y), (x',y',z'), g;reflexivity.
-        + destruct x,y; try (destruct x); try (destruct y); inversion H.
-  - inversion H.
-  - inversion H.
-  - inversion H.
-  - right. right. right. right. right. right. right. right. right. reflexivity.
-  - right. right. right. right. right. right. right. right. right. reflexivity.
-  - right. right. right. right. right. right. right. right. right. reflexivity.
+  - destruct d;inversion H.
+  - right. right. right. right. right. reflexivity.
 Qed.
 
 Proposition for_all_correct_physical :
@@ -778,69 +127,44 @@ Proposition for_all_correct_physical :
 .
 Proof.
   induction e; intros;simpl in *; try (exfalso; apply H; reflexivity).
-  - destruct d.
-    + simpl. clear H. generalize dependent m. induction Warp_size; intros. apply H0. simpl in *. inversion H0;subst.
-    apply cons_eq. apply IHn. apply H4. apply cons_neq. apply IHn. apply H4. apply Hneq.
-    + exfalso; apply H; reflexivity.
-    + exfalso; apply H; reflexivity.
-  - destruct shp as [[x y] z]. destruct id as [[id idy] idz]. destruct d.
-    + destruct x,y,z.
-      * apply H0.
-      * destruct z; apply H0.
-      * destruct y; apply H0.
-      * destruct y; destruct z; apply H0.
-      * destruct x. apply H0. clear H. simpl. clear b. induction x. apply H0. apply IHx.
-      * destruct x. destruct z; apply H0. clear H. destruct z; simpl; clear b; induction x; try apply H0; apply IHx.
-      * destruct x. destruct y; apply H0. clear H. destruct y; simpl; clear b; induction x; try apply H0; apply IHx.
-      * destruct x. destruct y,z; apply H0. clear H. destruct y,z; simpl; clear b; induction x; try apply H0; apply IHx.
-    + destruct y,x,z.
-      * apply H0.
-      * destruct z; apply H0.
-      * destruct x; apply H0.
-      * destruct x; destruct z; apply H0.
-      * destruct y. apply H0. clear H. simpl. clear b. induction y. apply H0. apply IHy.
-      * destruct y. destruct z; apply H0. clear H. destruct z; simpl; clear b; induction y; try apply H0; apply IHy.
-      * destruct y. destruct x; apply H0. clear H. destruct x; simpl; clear b; induction y; try apply H0; apply IHy.
-      * destruct y. destruct x,z; apply H0. clear H. destruct x,z; simpl; clear b; induction y; try apply H0; apply IHy.
-    + destruct z,x,y.
-      * apply H0.
-      * destruct y; apply H0.
-      * destruct x; apply H0.
-      * destruct x; destruct y; apply H0.
-      * destruct z. apply H0. clear H. simpl. clear b. induction z. apply H0. apply IHz.
-      * destruct z. destruct y; apply H0. clear H. destruct y; simpl; clear b; induction z; try apply H0; apply IHz.
-      * destruct z. destruct x; apply H0. clear H. destruct x; simpl; clear b; induction z; try apply H0; apply IHz.
-      * destruct z. destruct x,y; apply H0. clear H. destruct x,y; simpl; clear b; induction z; try apply H0; apply IHz.
-  - destruct shp as [[x y] z]. destruct shp' as [[x' y'] z']. destruct d.
-    + destruct x,y,z.
-      * apply H0.
-      * destruct z; apply H0.
-      * destruct y; apply H0.
-      * destruct y; destruct z; apply H0.
-      * destruct x. apply H0. clear H. simpl. clear g. induction x. apply H0. apply IHx.
-      * destruct x. destruct z; apply H0. clear H. destruct z; simpl; clear g; induction x; try apply H0; apply IHx.
-      * destruct x. destruct y; apply H0. clear H. destruct y; simpl; clear g; induction x; try apply H0; apply IHx.
-      * destruct x. destruct y,z; apply H0. clear H. destruct y,z; simpl; clear g; induction x; try apply H0; apply IHx.
-    + destruct y,x,z.
-      * apply H0.
-      * destruct z; apply H0.
-      * destruct x; apply H0.
-      * destruct x; destruct z; apply H0.
-      * destruct y. apply H0. clear H. simpl. clear g. induction y. apply H0. apply IHy.
-      * destruct y. destruct z; apply H0. clear H. destruct z; simpl; clear g; induction y; try apply H0; apply IHy.
-      * destruct y. destruct x; apply H0. clear H. destruct x; simpl; clear g; induction y; try apply H0; apply IHy.
-      * destruct y. destruct x,z; apply H0. clear H. destruct x,z; simpl; clear g; induction y; try apply H0; apply IHy.
-    + destruct z,x,y.
-      * apply H0.
-      * destruct y; apply H0.
-      * destruct x; apply H0.
-      * destruct x; destruct y; apply H0.
-      * destruct z. apply H0. clear H. simpl. clear g. induction z. apply H0. apply IHz.
-      * destruct z. destruct y; apply H0. clear H. destruct y; simpl; clear g; induction z; try apply H0; apply IHz.
-      * destruct z. destruct x; apply H0. clear H. destruct x; simpl; clear g; induction z; try apply H0; apply IHz.
-      * destruct z. destruct x,y; apply H0. clear H. destruct x,y; simpl; clear g; induction z; try apply H0; apply IHz.
   - apply induction_step_collection_forall_physical. intros.
     apply H with (n := n') (m := n0) (f := f) in H0.
     apply H0. apply H2. apply H3. apply H1.
+  - destruct d.
+    + simpl in *. clear H. clear H0.
+      generalize dependent m. induction x.
+      * intros. apply H1.
+      * intros. simpl in *. rewrite cat_empty. apply cat_count_rev in H1.
+      destruct H1 as [m1 [m2 [H1 [H2 H3]]]]; subst.
+      apply cat_count. apply H1. apply IHx. apply H2.
+    + simpl in *. apply transpose_lemma. clear H. clear H0.
+      generalize dependent m. induction x.
+      * intros. apply H1.
+      * intros. simpl in *. apply cat_count_rev in H1.
+      destruct H1 as [m1 [m2 [H1 [H2 H3]]]]; subst.
+      apply cat_count. clear H2. clear IHx.
+        generalize dependent m1. induction y. intros.
+            apply H1. intros. apply cat_count_rev in H1.
+        destruct H1 as [m1' [m2' [H1 [H2 H3]]]]; subst.
+        apply cat_count. rewrite cat_empty. apply H1. apply IHy.
+        apply H2.
+      apply IHx. apply H2.
+    + simpl in *. apply transpose_lemma. apply transpose_lemma'. clear H. clear H0.
+      generalize dependent m. induction x.
+      * intros. apply H1.
+      * intros. simpl in *. apply cat_count_rev in H1.
+      destruct H1 as [m1 [m2 [H1 [H2 H3]]]]; subst.
+      apply cat_count. clear H2. clear IHx.
+        generalize dependent m1. induction y. intros.
+          apply H1. intros. apply cat_count_rev in H1.
+          destruct H1 as [m1' [m2' [H1 [H2 H3]]]]; subst.
+          apply cat_count. clear H2. clear IHy.
+          generalize dependent m1'. induction z. intros.
+            apply H1. intros. apply cat_count_rev in H1.
+            destruct H1 as [m1'' [m2'' [H1 [H2 H3]]]]; subst.
+            apply cat_count. rewrite cat_empty. apply H1. apply IHz.
+            apply H2.
+        apply IHy. apply H2.
+      apply IHx. apply H2.
 Qed.
 
